---
header-includes:
- \usepackage{amssymb, amsmath, amsthm}
- \usepackage{tabu}
- \newcommand{\E}{\mathbb{E}}
- \newcommand{\var}{{\rm Var}}
- \newcommand{\N}{\mathcal{N}}
output: pdf_document
---

\noindent \begin{tabu} to \textwidth {@{}X[4 l] @{}X[r]}
  \textbf{HW 2}           & \\ 
  \textbf{MFE 403: Stochastic Calculus}   & \\ 
  \textbf{Professor Stavros Panageas}         & \\
  \textbf{Group 6}          &\\
  \textbf{Students: Xiahao Wang, Juan Manuel Ferreyra Maspero, Xinyue Zhu, Yichu Li, Mu Lin}
\end{tabu}


## Problem 1

Let $Z_s = W_s^3$

Apply Ito's lemma to get:

$$dZ_s = 3W_s^2dW_s + \frac{1}{2} \cdot 6W_s(dW_s)^2$$
Given:
$$Z(0) = 0$$

Integrate on both sides to get:

$$\int_0^tdZ_s = W_t^3$$
$$W_t^3 = 3\int_0^tW_s^2dW_s + W_sds$$
$$\int_0^tW_s^2dW_s = \frac{1}{3}W_t^3 - \int_0^tW_sds$$

## Problem 2 

$$X(t) = W_1(t) \times W_2(t)$$
Fix any $u < t$, we have
$$E[X_t |\mathcal{F}_u] = E[W_1(t) \times W_2(t) | \mathcal{F}_u]$$
$$= E[W_1(t)|\mathcal{F}_u] \times E[W_2(t)|\mathcal{F}_u] $$
$$ = W_1(u) \times W_2(u) = X(u)$$
Hence it is a martingale

## Problem 3
$$X_t = \int_0^t g(s)dW_s$$
$$dX_t = g(t)W_t$$
$$Z_t = e^{-\frac{\eta^2}{2}\int_0^tg^2(s)ds + \eta\int_0^tg(s)dW_s}$$
Apply Ito's Lemma:
$$dZ_t = -\frac{\eta^2}{2}g^2(t)dt\cdot Z_t + \eta g(t)dW_t \cdot Z_t + \frac{\eta^2}{2}g^2(t)dtZ_t$$
$$dZ_t = \eta g(t)dW_t \cdot Z_t =\eta dX_t \cdot Z_t $$
$$Z(0) =1$$
$$E[\int_0^tdZ_t] = E[\int_0^t\eta dX_s \cdot Z_s]$$
$$E[Z_t - Z(0)] = E[\int_0^t\eta g(s)dW_sZ_s] = \eta \sum_{k=0}^{n-1} E[g(t_k)E_{t_k}[W(t_{k+1})-W(t_{k})] \cdot Z_k]$$
hence $$ E[Z_t] = 1 = Z(0)$$ 
It is a martingale
$$E[Z_t] = e^{-\frac{\eta^2}{2}\int_0^tg^2(s)ds }E[e^{\eta\int_0^tg(s)dW_s}] = 1$$
$$E[e^{\eta\int_0^tg(s)dW_s}] = e^{\frac{\eta^2}{2}\int_0^tg^2(s)ds} $$
$$E[e^{\eta X_t}] = e^{\frac{\eta^2}{2}\int_0^tg^2(s)ds}$$
Based on the Moment Generating function, the Standard Deviation should be: $$\sqrt{\int_0^tg^2(s)ds}$$

## Problem 4

$$Z_t = W_t^k$$
Apply Ito's Lemma
$$dZ_t = 0 \cdot dt + kW_t^{k-1}dW_t + \frac{1}{2}[k(k-1)W_t^{k-2}(dW_t)^2]$$
$$=kW_t^{k-1}dW_t + \frac{1}{2}[k(k-1)W_t^{k-2}dt]$$
$Z_0 = 0$
$$\int_0^tdZ_s = Z_t = W_t^k$$ 
$$W_t^k = \int_0^tkW^{k-1}dW_s + \frac{1}{2}k(k-1)W_s^{k-2}ds$$

$$B_k(t) = E[Z_t] = E[W_t^k]$$

$$= E[\int_0^tkW^{k-1}dW_s + \frac{1}{2}k(k-1)W_s^{k-2}ds]$$

$$ =  0 + \frac{1}{2}k(k-1)\int_0^tE[W_s^{k-2}]ds$$
$$ = \frac{1}{2}k(k-1)\int_0^tB_{k-2}(s)ds$$
